RocqOfRust/revm/revm_interpreter/instructions/contract/links/call_helpers.v
@@ -1,4 +1,6 @@
 Require Import links.RocqOfRust.
+Require Import alloy_primitives.bits.links.address.
+Require Import alloy_primitives.bits.links.fixed_FixedBytes.
 Require Import alloy_primitives.bytes.links.mod.
 Require Import alloy_primitives.links.aliases.
 Require Import core.convert.links.mod.
@@ -6,16 +8,86 @@ Require Import core.links.cmp.
 Require Import core.links.option.
 Require Import core.num.links.mod.
 Require Import core.ops.links.range.
+Require Import revm.revm_bytecode.links.bytecode.
 Require Import revm.revm_context_interface.links.journaled_state.
 Require Import revm.revm_interpreter.gas.links.calc.
 Require Import revm.revm_interpreter.instructions.contract.call_helpers.
 Require Import revm.revm_interpreter.interpreter.links.shared_memory.
 Require Import revm.revm_interpreter.links.gas.
+Require Import revm.revm_interpreter.links.instruction_context.
 Require Import revm.revm_interpreter.links.instruction_result.
 Require Import revm.revm_interpreter.links.interpreter.
 Require Import revm.revm_interpreter.links.interpreter_types.
 Require Import revm.revm_primitives.links.hardfork.
 Require Import ruint.links.lib.
+
+#[export] Existing Instance Option.IsLink.
+#[export] Existing Instance FixedBytes.IsLink.
+
+Module LoadAccAndCalcGasResult.
+  Record t : Set := {
+    gas_limit : u64;
+    bytecode : Bytecode.t;
+    bytecode_hash : aliases.B256.t;
+  }.
+
+  Global Instance IsLink : Link t := {
+    Φ := Ty.tuple [
+      Φ u64;
+      Φ Bytecode.t;
+      Φ aliases.B256.t
+    ];
+    φ x := Value.Tuple [
+      φ x.(gas_limit);
+      φ x.(bytecode);
+      φ x.(bytecode_hash)
+    ];
+  }.
+
+  Definition of_ty :
+    OfTy.t (Ty.tuple [
+      Φ u64;
+      Φ Bytecode.t;
+      Φ aliases.B256.t
+    ]).
+  Proof. eapply OfTy.Make with (A := t); reflexivity. Defined.
+  Smpl Add apply of_ty : of_ty.
+
+  Module SubPointer.
+    Definition get_gas_limit : SubPointer.Runner.t t (Pointer.Index.Tuple 0) :=
+    {|
+      SubPointer.Runner.projection x := Some x.(gas_limit);
+      SubPointer.Runner.injection x y := Some (x <| gas_limit := y |>);
+    |}.
+
+    Lemma get_gas_limit_is_valid :
+      SubPointer.Runner.Valid.t get_gas_limit.
+    Proof. now constructor. Qed.
+    Smpl Add apply get_gas_limit_is_valid : run_sub_pointer.
+
+    Definition get_bytecode : SubPointer.Runner.t t (Pointer.Index.Tuple 1) :=
+    {|
+      SubPointer.Runner.projection x := Some x.(bytecode);
+      SubPointer.Runner.injection x y := Some (x <| bytecode := y |>);
+    |}.
+
+    Lemma get_bytecode_is_valid :
+      SubPointer.Runner.Valid.t get_bytecode.
+    Proof. now constructor. Qed.
+    Smpl Add apply get_bytecode_is_valid : run_sub_pointer.
+
+    Definition get_bytecode_hash : SubPointer.Runner.t t (Pointer.Index.Tuple 2) :=
+    {|
+      SubPointer.Runner.projection x := Some x.(bytecode_hash);
+      SubPointer.Runner.injection x y := Some (x <| bytecode_hash := y |>);
+    |}.
+
+    Lemma get_bytecode_hash_is_valid :
+      SubPointer.Runner.Valid.t get_bytecode_hash.
+    Proof. now constructor. Qed.
+    Smpl Add apply get_bytecode_hash_is_valid : run_sub_pointer.
+  End SubPointer.
+End LoadAccAndCalcGasResult.
 
 (*
 pub fn resize_memory(
@@ -84,3 +156,28 @@ Proof.
   ].
 Defined.
 Global Opaque run_get_memory_input_and_out_ranges.
+
+(*
+pub fn load_acc_and_calc_gas<H: Host + ?Sized>(
+    context: &mut InstructionContext<'_, H, impl InterpreterTypes>,
+    to: Address,
+    transfers_value: bool,
+    create_empty_account: bool,
+    stack_gas_limit: u64,
+) -> Option<(u64, Bytecode, B256)>
+*)
+Instance run_load_acc_and_calc_gas
+  {WIRE H : Set} `{Link WIRE} `{Link H}
+  {WIRE_types : InterpreterTypes.Types.t} `{InterpreterTypes.Types.AreLinks WIRE_types}
+  (context : '&mut (InstructionContext.t H WIRE WIRE_types))
+  (to : Address.t)
+  (transfers_value create_empty_account : bool)
+  (stack_gas_limit : u64) :
+  Run.Trait
+    instructions.contract.call_helpers.load_acc_and_calc_gas
+    [] [Φ H; Φ WIRE]
+    [φ context; φ to; φ transfers_value; φ create_empty_account; φ stack_gas_limit]
+    (option LoadAccAndCalcGasResult.t).
+Proof.
+Admitted.
+Global Opaque run_load_acc_and_calc_gas.
