RocqOfRust/revm/revm_interpreter/instructions/contract/simulate/call_helpers.v
@@ -1,4 +1,5 @@
 Require Import simulate.RocqOfRust.
+Require Import alloy_primitives.bits.links.address.
 Require Import alloy_primitives.bytes.links.mod.
 Require Import alloy_primitives.bytes.simulate.mod.
 Require Import alloy_primitives.links.aliases.
@@ -7,12 +8,17 @@ Require Import core.num.simulate.mod.
 Require Import core.ops.links.range.
 Require Import core.ops.simulate.deref.
 Require Import core.ops.simulate.range.
+Require Import revm.revm_bytecode.links.bytecode.
+Require Import revm.revm_context_interface.links.host.
 Require Import revm.revm_context_interface.links.journaled_state.
+Require Import revm.revm_context_interface.simulate.host.
 Require Import revm.revm_interpreter.gas.simulate.calc.
+Require Import revm.revm_interpreter.gas.simulate.constants.
 Require Import revm.revm_interpreter.instructions.contract.links.call_helpers.
 Require Import revm.revm_interpreter.instructions.simulate.macros.
 Require Import revm.revm_interpreter.interpreter.simulate.shared_memory.
 Require Import revm.revm_interpreter.links.gas.
+Require Import revm.revm_interpreter.links.instruction_context.
 Require Import revm.revm_interpreter.links.interpreter.
 Require Import revm.revm_interpreter.links.interpreter_types.
 Require Import revm.revm_interpreter.simulate.gas.
@@ -20,6 +26,9 @@ Require Import revm.revm_interpreter.simulate.interpreter_types.
 Require Import revm.revm_primitives.links.hardfork.
 Require Import revm.revm_primitives.simulate.hardfork.
 Require Import ruint.simulate.lib.
+
+Parameter bytecode_of_account_load : AccountLoad.t -> Bytecode.t.
+Parameter bytecode_hash_of_account_load : AccountLoad.t -> aliases.B256.t.
 
 Definition resize_memory
     {WIRE : Set} `{Link WIRE}
@@ -133,7 +142,7 @@ Definition get_memory_input_and_out_ranges
     {WIRE_types : InterpreterTypes.Types.t} `{InterpreterTypes.Types.AreLinks WIRE_types}
     {IInterpreterTypes : InterpreterTypes.C WIRE_types}
     (interpreter : Interpreter.t WIRE WIRE_types) :
-    option (Bytes.t * Range.t usize) * Interpreter.t WIRE WIRE_types :=
+    option (Range.t usize * Range.t usize) * Interpreter.t WIRE WIRE_types :=
   popn_macro interpreter {| Integer.value := 4 |}
     (fun interpreter => (None, interpreter))
     (fun arr interpreter =>
@@ -144,28 +153,25 @@ Definition get_memory_input_and_out_ranges
   | None => (None, interpreter)
   | Some in_range =>
 
-  let input :=
+  let in_range :=
     if Impl_Range.is_empty in_range then
-      Impl_Bytes.new
+      in_range
     else
-      let slice :=
-        IInterpreterTypes.(InterpreterTypes.MemoryTrait_for_Memory).(MemoryTrait.slice)
-            interpreter.(Interpreter.memory)
-            in_range in
-      let slice : list u8 :=
+      let offset :=
         IInterpreterTypes
           .(InterpreterTypes.MemoryTrait_for_Memory)
-          .(MemoryTrait.Deref_for_Synthetic)
-          .(Deref.deref)
-          .(RefStub.projection)
-          slice in
-      Impl_Bytes.copy_from_slice slice in
+          .(MemoryTrait.local_memory_offset)
+          interpreter.(Interpreter.memory) in
+      {|
+        Range.start := Impl_usize.saturating_add in_range.(Range.start) offset;
+        Range.end_ := Impl_usize.saturating_add in_range.(Range.end_) offset;
+      |} in
 
   let '(ret_range_opt, interpreter) := resize_memory interpreter out_offset out_len in
   match ret_range_opt with
   | None => (None, interpreter)
   | Some ret_range =>
-  (Some (input, ret_range), interpreter)
+  (Some (in_range, ret_range), interpreter)
 
   end end).
 
@@ -200,20 +206,43 @@ Proof.
   cw @resize_memory_eq. *)
 Admitted.
 
-Definition calc_call_gas
-    {WIRE : Set} `{Link WIRE}
+Definition load_acc_and_calc_gas
+    {WIRE H : Set} `{Link WIRE} `{Link H}
     {WIRE_types : InterpreterTypes.Types.t} `{InterpreterTypes.Types.AreLinks WIRE_types}
     {IInterpreterTypes : InterpreterTypes.C WIRE_types}
-    {IRuntimeFlag : RuntimeFlag.C WIRE_types.(InterpreterTypes.Types.RuntimeFlag)}
+    {H_types : Host.Types.t} `{Host.Types.AreLinks H_types}
+    {IHost : Host.C H H_types}
     (interpreter : Interpreter.t WIRE WIRE_types)
-    (account_load : AccountLoad.t)
-    (has_transfer : bool)
-    (local_gas_limit : u64) :
-    option u64 * Interpreter.t WIRE WIRE_types :=
-  let spec_id := IRuntimeFlag.(RuntimeFlag.spec_id) interpreter.(Interpreter.runtime_flag) in
-  let call_cost := call_cost spec_id has_transfer account_load in
-  gas_macro interpreter call_cost
-    (fun interpreter => (None, interpreter))
+    (host : H)
+    (to : Address.t)
+    (transfers_value create_empty_account : bool)
+    (stack_gas_limit : u64) :
+    option LoadAccAndCalcGasResult.t * Interpreter.t WIRE WIRE_types * H :=
+  let spec_id :=
+    IInterpreterTypes
+      .(InterpreterTypes.RuntimeFlag_for_RuntimeFlag)
+      .(RuntimeFlag.spec_id)
+      interpreter.(Interpreter.runtime_flag) in
+  let static_gas := calc_call_static_gas spec_id transfers_value in
+  gas_macro interpreter static_gas
+    (fun interpreter => (None, interpreter, host))
+    (fun interpreter =>
+
+  match IHost.(Host.load_account_delegated) host to with
+  | (None, host) =>
+    let control :=
+      IInterpreterTypes
+          .(InterpreterTypes.LoopControl_for_Control)
+          .(LoopControl.set_instruction_result)
+        interpreter.(Interpreter.control)
+        instruction_result.InstructionResult.FatalExternalError in
+    let interpreter := interpreter <| Interpreter.control := control |> in
+    (None, interpreter, host)
+  | (Some account_load, host) =>
+
+  let dynamic_gas := warm_cold_cost_with_delegation account_load.(AccountLoad.load) in
+  gas_macro interpreter dynamic_gas
+    (fun interpreter => (None, interpreter, host))
     (fun interpreter =>
 
   let gas_limit :=
@@ -225,40 +254,83 @@ Definition calc_call_gas
           .(RefStub.projection)
           interpreter.(Interpreter.control) in
       let remaining := Impl_Gas.remaining_63_of_64_parts gas in
-      Z.min i[remaining] i[local_gas_limit] : u64
+      Z.min i[remaining] i[stack_gas_limit] : u64
     else
-      local_gas_limit in
+      stack_gas_limit in
+  gas_macro interpreter gas_limit
+    (fun interpreter => (None, interpreter, host))
+    (fun interpreter =>
 
-  (Some gas_limit, interpreter)
-  ).
+  let gas_limit :=
+    if transfers_value then
+      Impl_u64.saturating_add gas_limit CALL_STIPEND
+    else
+      gas_limit in
+  (
+    Some {|
+      LoadAccAndCalcGasResult.gas_limit := gas_limit;
+      LoadAccAndCalcGasResult.bytecode := bytecode_of_account_load account_load;
+      LoadAccAndCalcGasResult.bytecode_hash := bytecode_hash_of_account_load account_load;
+    |},
+    interpreter,
+    host
+  ))) end).
 
-Lemma calc_call_gas_eq
-    {WIRE : Set} `{Link WIRE}
+Lemma load_acc_and_calc_gas_eq
+    {WIRE H : Set} `{Link WIRE} `{Link H}
     {WIRE_types : InterpreterTypes.Types.t} `{InterpreterTypes.Types.AreLinks WIRE_types}
+    {H_types : Host.Types.t} `{Host.Types.AreLinks H_types}
     (run_InterpreterTypes_for_WIRE : InterpreterTypes.Run WIRE WIRE_types)
+    (run_Host_for_H : Host.Run H H_types)
     `{IInterpreterTypes : !InterpreterTypes.C WIRE_types}
     `{InterpreterTypesEq :
       !InterpreterTypes.Eq.t WIRE WIRE_types run_InterpreterTypes_for_WIRE IInterpreterTypes}
+    `{IHost : !Host.C H H_types}
+    `{HostEq : !Host.Eq.t IHost}
     (interpreter : Interpreter.t WIRE WIRE_types)
-    (account_load : AccountLoad.t)
-    (has_transfer : bool)
-    (local_gas_limit : u64)
+    (host : H)
+    (to : Address.t)
+    (transfers_value create_empty_account : bool)
+    (stack_gas_limit : u64)
     (stack : Stack.t) :
-  let ref_interpreter := make_ref 0 in
+  let ref_context := make_ref (A := InstructionContext.t H WIRE WIRE_types) 0 in
+  let ref_interpreter := make_ref (A := Interpreter.t WIRE WIRE_types) 1 in
+  let ref_host := make_ref (A := H) 2 in
+  let context := {|
+    InstructionContext.interpreter := ref_interpreter;
+    InstructionContext.host := ref_host;
+  |} in
   {{
     SimulateM.eval_f (
-      run_calc_call_gas
-        run_InterpreterTypes_for_WIRE
-        ref_interpreter
-        account_load
-        has_transfer
-        local_gas_limit
+      run_load_acc_and_calc_gas
+        ref_context
+        to
+        transfers_value
+        create_empty_account
+        stack_gas_limit
     )
-    (interpreter :: stack)%stack 🌲
-    let result_interpreter := calc_call_gas interpreter account_load has_transfer local_gas_limit in
+    (context :: interpreter :: host :: stack)%stack 🌲
+    let '(result, interpreter, host) :=
+      @load_acc_and_calc_gas
+        WIRE
+        H
+        H0
+        H1
+        WIRE_types
+        H2
+        IInterpreterTypes
+        H_types
+        H3
+        IHost
+        interpreter
+        host
+        to
+        transfers_value
+        create_empty_account
+        stack_gas_limit in
     (
-      Output.Success (fst result_interpreter),
-      (snd result_interpreter :: stack)%stack
+      Output.Success result,
+      (context :: interpreter :: host :: stack)%stack
     )
   }}.
 Proof.
